theories/Bisim.v
@@ -722,3 +722,8 @@ Tactic Notation "coinduction" simple_intropattern(R) simple_intropattern(H) :=
 
 #[global] Opaque wtrans.
 
+Ltac eq2equ H :=
+  match type of H with
+  | ?u = ?t => let eq := fresh "EQ" in assert (eq : u ≅ t) by (subst; reflexivity); clear H
+  end.
+
